theories/string_lang/StringLangExamples.v
@@ -23,4 +23,7 @@ Check (prg : program).
 Lemma prg_string_1 : program_over prg 1.
 Proof.
   split; simpl; auto.
-Qed.
+Qed. 
+
+
+
